formal-proofs/theories/lib/concurrent_linked_list/infinite_array/array_spec.v
@@ -9,64 +9,81 @@ Record infiniteArraySpec Σ `{!heapG Σ} :=
       derefCellPointer: val;
       cutoffMoveForward: val;
       cutoffGetPointer: val;
+      cellPointerId: val;
       infinite_array_name: Type;
       is_infinite_array (N: namespace) (γ: infinite_array_name)
                         (cell_is_owned: nat → iProp Σ): iProp Σ;
       is_infinite_array_persistent N γ co:
         Persistent (is_infinite_array N γ co);
-      infinite_array_mapsto (γ: infinite_array_name) (i: nat) (ℓ: loc): iProp Σ;
-      infinite_array_mapsto_persistent γ i ℓ:
-        Persistent (infinite_array_mapsto γ i ℓ);
-      infinite_array_mapsto_agree γ i ℓ ℓ':
-        infinite_array_mapsto γ i ℓ -∗ infinite_array_mapsto γ i ℓ' -∗ ⌜ℓ = ℓ'⌝;
-      is_infinite_array_cell_pointer (γ: infinite_array_name) (p: val) (i: nat):
+      infinite_array_mapsto (N: namespace) (cell_is_owned: nat -> iProp Σ)
+                            (γ: infinite_array_name) (i: nat) (ℓ: loc): iProp Σ;
+      infinite_array_mapsto_persistent N co γ i ℓ:
+        Persistent (infinite_array_mapsto N co γ i ℓ);
+      infinite_array_mapsto_agree N co γ i ℓ ℓ':
+        infinite_array_mapsto N co γ i ℓ -∗ infinite_array_mapsto N co γ i ℓ'
+                              -∗ ⌜ℓ = ℓ'⌝;
+      is_infinite_array_cell_pointer N (γ: infinite_array_name) (p: val) (i: nat):
           iProp Σ;
-      is_infinite_array_cell_pointer_persistent γ p i:
-        Persistent (is_infinite_array_cell_pointer γ p i);
-      is_infinite_array_cutoff
+      is_infinite_array_cutoff_reading (N: namespace) (γ: infinite_array_name)
+                                       (p: val) (start_id: nat): iProp Σ;
+      is_infinite_array_cell_pointer_persistent N γ p i:
+        Persistent (is_infinite_array_cell_pointer N γ p i);
+      is_infinite_array_cutoff (N: namespace)
         (γ: infinite_array_name) (v: val) (start_index: nat): iProp Σ;
-      cell_is_cancelled (γ: infinite_array_name) (i: nat): iProp Σ;
-      cell_is_cancelled_persistent γ i: Persistent (cell_is_cancelled γ i);
-      cell_cancellation_handle (γ: infinite_array_name) (i: nat): iProp Σ;
-      cell_cancellation_handle_exclusive γ i:
-        cell_cancellation_handle γ i -∗ cell_cancellation_handle γ i -∗ False;
-      cell_cancellation_handle_not_cancelled γ i:
-        cell_is_cancelled γ i -∗ cell_cancellation_handle γ i -∗ False;
-      acquire_cell N γ cell_is_owned i ℓ:
-        is_infinite_array N γ cell_is_owned -∗
-        infinite_array_mapsto γ i ℓ -∗
-        ∀ Φ, (cell_is_owned i ∨ ℓ ↦ NONEV ∗ cell_cancellation_handle γ i
-                                ={⊤∖↑N}=∗ cell_is_owned i ∗ Φ) ==∗ Φ;
+      cell_is_cancelled (N: namespace) (γ: infinite_array_name) (i: nat): iProp Σ;
+      cell_is_cancelled_persistent N γ i: Persistent (cell_is_cancelled N γ i);
+      cell_cancellation_handle
+        (N: namespace) (γ: infinite_array_name) (i: nat): iProp Σ;
+      cell_cancellation_handle_exclusive N γ i:
+        cell_cancellation_handle N γ i -∗ cell_cancellation_handle N γ i -∗ False;
+      cell_cancellation_handle_not_cancelled N γ i:
+        cell_is_cancelled N γ i -∗ cell_cancellation_handle N γ i -∗ False;
+      acquire_cell N cell_is_owned E γ i ℓ:
+        ↑N ⊆ E →
+        infinite_array_mapsto N cell_is_owned γ i ℓ ={E, E∖↑N}=∗
+        ▷ (cell_is_owned i ∨ ℓ ↦ NONEV ∗ cell_cancellation_handle N γ i) ∗
+        (▷ cell_is_owned i ={E∖↑N, E}=∗ True);
+      newInfiniteArray_spec N co k:
+        {{{ ⌜(k > 0)%nat⌝ ∧ inv_heap_inv }}}
+          newInfiniteArray #k
+        {{{ γ ℓ, RET #ℓ; is_infinite_array N γ co ∗
+                        [∗ list] i ∈ seq 0 k,
+                          is_infinite_array_cutoff N γ #(ℓ +ₗ Z.of_nat i) 0
+        }}};
       cancelCell_spec N γ co p i:
         is_infinite_array N γ co -∗
-        is_infinite_array_cell_pointer γ p i -∗
-        <<< cell_cancellation_handle γ i >>>
-            cancelCell p @ ⊤
-        <<< cell_is_cancelled γ i, RET #() >>>;
+        is_infinite_array_cell_pointer N γ p i -∗
+        <<< cell_cancellation_handle N γ i >>>
+            cancelCell p @ ⊤ ∖ ↑N
+        <<< cell_is_cancelled N γ i, RET #() >>>;
       findCell_spec N γ co p (source_id id: nat):
         {{{ is_infinite_array N γ co ∗
-            is_infinite_array_cell_pointer γ p source_id }}}
+            is_infinite_array_cutoff_reading N γ p source_id }}}
         findCell p #id @ ⊤
-        {{{ p' id', RET p'; is_infinite_array_cell_pointer γ p' id'
-            ∗ (⌜source_id <= id <= id'⌝ ∨
-              ⌜source_id > id ∧ id' = source_id⌝)%nat
-            ∗ [∗ list] i ∈ seq id (id' - id), cell_is_cancelled γ i
+        {{{ p' id', RET p'; is_infinite_array_cell_pointer N γ p' id'
+            ∗ ⌜(id ≤ id')%nat⌝
+            ∗ ∀ i, (⌜max source_id id ≤ i < id'⌝)%nat -∗ cell_is_cancelled N γ i
         }}};
-      derefCellPointer_spec γ (p: val) i:
-        {{{ is_infinite_array_cell_pointer γ p i }}}
+      derefCellPointer_spec N co γ (p: val) i:
+        {{{ is_infinite_array N γ co ∗ is_infinite_array_cell_pointer N γ p i }}}
           derefCellPointer p
-        {{{ ℓ, RET #ℓ; infinite_array_mapsto γ i ℓ }}};
-      cutoffMoveForward_spec γ (p v: val) i:
-        is_infinite_array_cell_pointer γ p i -∗
-        <<< ∀ start_index, ▷ is_infinite_array_cutoff γ v start_index >>>
-          cutoffMoveForward v p @ ⊤
+        {{{ ℓ, RET #ℓ; infinite_array_mapsto N co γ i ℓ }}};
+      cutoffMoveForward_spec N co γ (p v: val) i:
+        is_infinite_array N γ co -∗
+        is_infinite_array_cell_pointer N γ p i -∗
+        <<< ∀ start_index, ▷ is_infinite_array_cutoff N γ v start_index >>>
+          cutoffMoveForward v p @ ⊤ ∖ ↑N
         <<< ∃ (success: bool), if success
-            then ∃ i', ⌜start_index ≤ i' ≤ i⌝ ∧ is_infinite_array_cutoff γ v i'
-            else ▷ is_infinite_array_cutoff γ v start_index ∗
-                cell_is_cancelled γ start_index, RET #success >>>;
-      cutoffGetPointer_spec γ (v: val):
-        ⊢ <<< ∀ i, ▷ is_infinite_array_cutoff γ v i >>>
+            then ∃ i', ⌜start_index ≤ i' ≤ max i start_index⌝ ∧
+                      is_infinite_array_cutoff N γ v i'
+            else ▷ is_infinite_array_cutoff N γ v start_index, RET #success >>>;
+      cutoffGetPointer_spec N γ (v: val):
+        ⊢ <<< ∀ i, ▷ is_infinite_array_cutoff N γ v i >>>
           cutoffGetPointer v @ ⊤
-        <<< ∃ (p: val), is_infinite_array_cutoff γ v i ∗
-                        is_infinite_array_cell_pointer γ p i, RET p >>>
+        <<< ∃ (p: val), is_infinite_array_cutoff N γ v i ∗
+                        is_infinite_array_cutoff_reading N γ p i, RET p >>>;
+      cellPointerId_spec N co γ (p: val) i:
+        {{{ is_infinite_array N γ co ∗ is_infinite_array_cell_pointer N γ p i }}}
+          cellPointerId p
+        {{{ RET #i; True }}};
     }.
